src/goose_lang/prelude.v
@@ -2,7 +2,7 @@ From Perennial.goose_lang Require Export lang notation typing.
 From Perennial.goose_lang.lib Require Export
      typed_mem.impl struct.impl loop.impl
      encoding.impl map.impl slice.impl lock.impl
-     time.impl proph.impl.
+     time.impl proph.impl waitgroup.impl.
 
 (* We provide stubs here for primitive operations to make the Goose unit tests
    compile. *)
