src/program_proof/simplepb/pb_definitions.v
@@ -1,0 +1,3 @@
+From Perennial.program_proof Require Import grove_prelude.
+From Goose.github_com.mit_pdos.gokv.simplepb Require Import pb client config admin.
+From Perennial.program_proof.grove_shared Require Import urpc_proof urpc_spec.
